GroupoidModel/Syntax/Env.lean
@@ -1,0 +1,127 @@
+import GroupoidModel.Syntax.Synth
+import GroupoidModel.Syntax.Typechecker.Value
+
+variable {χ : Type*} {E : Env χ}
+
+theorem isClosed_all :
+    (∀ {Γ l A}, E ∣ Γ ⊢[l] A → A.isClosed Γ.length) ∧
+    (∀ {Γ l A t}, E ∣ Γ ⊢[l] t : A → t.isClosed Γ.length) := by
+  mutual_induction WfTp
+  all_goals try exact True.intro
+  case bvar =>
+    intros; rename_i lk _
+    simp [Expr.isClosed, lk.lt_length]
+  all_goals grind [Expr.isClosed]
+
+theorem WfTp.isClosed {l A} : E ∣ [] ⊢[l] A → A.isClosed := isClosed_all.1
+theorem WfTm.isClosed {l A t} : E ∣ [] ⊢[l] t : A → t.isClosed := isClosed_all.2
+
+/-! ## Constant environments -/
+
+namespace Env
+
+def empty (χ) : Env χ := fun _ => none
+
+theorem Wf.empty (χ) : (empty χ).Wf := nofun
+
+open Classical
+
+instance : LE (Env χ) where
+  le E E' := ∀ ⦃c p⦄, (E c) = some p → (E' c) = some p
+
+noncomputable def snoc (E : Env χ)
+    (l : Nat) (c : χ) (A : Expr χ)
+    (l_le : l ≤ univMax) (A_cl : A.isClosed) : Env χ :=
+  fun d => if d = c then some ⟨(A, l), ⟨A_cl, l_le⟩⟩ else E d
+
+@[simp]
+theorem snoc_get (E : Env χ)
+    (l : Nat) (c : χ) (A : Expr χ)
+    (l_le : l ≤ univMax) (A_cl : A.isClosed) :
+    E.snoc l c A l_le A_cl c = some ⟨(A, l), ⟨A_cl, l_le⟩⟩ := by
+  simp [snoc]
+
+theorem le_snoc (E : Env χ)
+    (l : Nat) (c : χ) (A : Expr χ)
+    (l_le : l ≤ univMax) (A_cl : A.isClosed)
+    (Ec : E c = none) :
+    E ≤ E.snoc l c A l_le A_cl := by
+  intro d Al Ed
+  have : d ≠ c := by grind
+  simp only [snoc, this, ↓reduceIte, Ed]
+
+theorem _root_.of_env_le_all {E E' : Env χ} (le : E ≤ E') :
+    (∀ {Γ}, WfCtx E Γ → WfCtx E' Γ) ∧
+    (∀ {Γ l A}, E ∣ Γ ⊢[l] A → E' ∣ Γ ⊢[l] A) ∧
+    (∀ {Γ l A B}, E ∣ Γ ⊢[l] A ≡ B → E' ∣ Γ ⊢[l] A ≡ B) ∧
+    (∀ {Γ l A t}, E ∣ Γ ⊢[l] t : A → E' ∣ Γ ⊢[l] t : A) ∧
+    (∀ {Γ l A t u}, E ∣ Γ ⊢[l] t ≡ u : A → E' ∣ Γ ⊢[l] t ≡ u : A) := by
+  mutual_induction WfCtx
+  case const =>
+    intros; rename_i Ec Γ
+    apply WfTm.const Γ (le Ec)
+  grind_cases
+
+theorem Wf.snoc {E : Env χ} {A l}
+    (Ewf : E.Wf) (c : χ) (Awf : E ∣ [] ⊢[l] A) (Ec : E c = none) :
+    (E.snoc l c A Awf.le_univMax Awf.isClosed).Wf := by
+  intro d Al Ed
+  simp only [Env.snoc] at Ed
+  have le := E.le_snoc l c A Awf.le_univMax Awf.isClosed Ec
+  by_cases eq : d = c <;> simp only [eq, ↓reduceIte] at Ed
+  . cases Ed
+    exact of_env_le_all le |>.2.1 Awf
+  . exact of_env_le_all le |>.2.1 <| Ewf Ed
+
+end Env
+
+/-- An axiom checked with respect to the axioms in `E`. -/
+structure CheckedAx (E : Env χ) where
+  name : χ
+  get_name : E name = none
+  l : Nat
+  tp : Expr χ
+  nfTp : Val χ
+  wf_nfTp : ValEqTp E [] l nfTp tp
+
+namespace CheckedAx
+variable [Ewf : Fact E.Wf]
+
+theorem wf_tp (a : CheckedAx E) : E ∣ [] ⊢[a.l] a.tp :=
+  a.wf_nfTp.wf_tp
+
+/-- The set of axioms extended by this one. -/
+noncomputable def snocEnv (a : CheckedAx E) : Env χ :=
+  E.snoc a.l a.name a.tp a.wf_tp.le_univMax a.wf_tp.isClosed
+
+theorem wf_snocEnv (a : CheckedAx E) : a.snocEnv.Wf :=
+  Ewf.out.snoc a.name a.wf_tp a.get_name
+
+/-- The axiom as an expression. -/
+def val (a : CheckedAx E) : Expr χ :=
+  .const a.name
+
+theorem wf_val (a : CheckedAx E) : a.snocEnv ∣ [] ⊢[a.l] a.val : a.tp := by
+  unfold val
+  have := E.snoc_get a.l a.name a.tp a.wf_tp.le_univMax a.wf_tp.isClosed
+  apply WfTm.const .nil this
+
+end CheckedAx
+
+/-- A definition checked with respect to the axioms in `E`. -/
+structure CheckedDef (E : Env χ) where
+  l : Nat
+  tp : Expr χ
+  nfTp : Val χ
+  wf_nfTp : ValEqTp E [] l nfTp tp
+  val : Expr χ
+  -- nfVal?
+  wf_val : E ∣ [] ⊢[l] val : tp
+
+namespace CheckedDef
+variable [Fact E.Wf]
+
+theorem wf_tp (d : CheckedDef E) : E ∣ [] ⊢[d.l] d.tp :=
+  d.wf_val.wf_tp
+
+end CheckedDef
