GroupoidModel/Syntax/Frontend/Commands.lean
@@ -1,0 +1,147 @@
+import Lean
+import Qq
+import GroupoidModel.Syntax.Typechecker.Synth
+import GroupoidModel.Syntax.Frontend.EnvExt
+import GroupoidModel.Syntax.Frontend.Translation
+
+namespace Leanternal
+
+open Lean Elab Command
+open Qq
+
+def envDiff (old new : Environment) : Array ConstantInfo := Id.run do
+  let mut ret := #[]
+  for (c, i) in new.constants.map₂ do
+    if old.constants.map₂.contains c then continue
+    if c.isInternal then continue
+    ret := ret.push i
+  return ret
+
+def elabAxiom (thyNm : Name) (stx : Syntax) : CommandElabM Unit := do
+  let thyData ← getTheoryData thyNm
+  let thyEnv' ← withEnv thyData.env do Command.elabDeclaration stx; getEnv
+  if ← MonadLog.hasErrors then
+    return
+  let diff := envDiff thyData.env thyEnv'
+  let #[.axiomInfo ci] := diff
+    | throwError "expected exactly one axiom, got {diff.size}:\
+      {Lean.indentD ""}{diff.map (·.name)}"
+  Command.liftTermElabM do
+    let env ← getEnv
+    let (l, T) ← withEnv thyData.env <| translateAsTp ci.type |>.run env
+    trace[Leanternal.Translation]
+      "axiom.\{{l}} {ci.name} :\
+          {Lean.indentExpr T |>.nest 2}"
+
+    have axioms : Q(Env Name) := thyData.axioms
+    have wf_axioms : Q(($axioms).Wf) := thyData.wf_axioms
+    have name : Q(Name) := toExpr ci.name
+    -- TODO: smarter tactic for this equality
+    let ⟨_⟩ ← assertDefEqQ q($axioms $name) q(none)
+    let Twf ← checkTp q($axioms) q(⟨$wf_axioms⟩) q([]) q($l) q($T)
+    let ⟨vT, vTeq⟩ ← evalTpId q(show TpEnv Lean.Name from []) q($T)
+    let value : Q(CheckedAx $axioms) := q(
+      have : Fact ($axioms).Wf := ⟨$wf_axioms⟩
+      { name := $name
+        get_name := ‹_›
+        l := $l
+        tp := $T
+        nfTp := $vT
+        wf_nfTp := $vTeq .nil <| $Twf .nil
+      }
+    )
+
+    -- TODO: `addDeclQ`
+    addDecl <| .defnDecl {
+      name := ci.name
+      levelParams := []
+      type := q(CheckedAx $axioms)
+      value
+      hints := .regular 0 -- TODO: what height?
+      safety := .safe
+    }
+    have a : Q(CheckedAx $axioms) := .const ci.name []
+
+    saveShallowTheoryConst thyNm (.axiomInfo ci)
+    setTheoryData thyNm { thyData with
+      env := thyEnv'
+      axioms := q(have : Fact ($axioms).Wf := ⟨$wf_axioms⟩; ($a).snocEnv)
+      wf_axioms := q(have : Fact ($axioms).Wf := ⟨$wf_axioms⟩; ($a).wf_snocEnv)
+    }
+
+def elabDeclaration (thyNm : Name) (stx : Syntax) : CommandElabM Unit := do
+  let thyData ← getTheoryData thyNm
+  let thyEnv' ← withEnv thyData.env do Command.elabDeclaration stx; getEnv
+  if ← MonadLog.hasErrors then
+    return
+  let diff := envDiff thyData.env thyEnv'
+  let #[.defnInfo ci] := diff
+    | throwError "expected exactly one definition, got {diff.size}:\
+      {Lean.indentD ""}{diff.map (·.name)}"
+  Command.liftTermElabM do
+    let env ← getEnv
+    let (l, T) ← withEnv thyData.env <| translateAsTp ci.type |>.run env
+    let (k, t) ← withEnv thyData.env <| translateAsTm ci.value |>.run env
+     if l != k then throwError "internal error: inferred level mismatch"
+    trace[Leanternal.Translation]
+      "def.\{{l}} {ci.name} :\
+          {Lean.indentExpr T |>.nest 2}\n\
+      :=\
+        {Lean.indentExpr t}"
+
+    have axioms : Q(Env Name) := thyData.axioms
+    have wf_axioms : Q(($axioms).Wf) := thyData.wf_axioms
+    let Twf ← checkTp q($axioms) q(⟨$wf_axioms⟩) q([]) q($l) q($T)
+    let ⟨vT, vTeq⟩ ← evalTpId q(show TpEnv Lean.Name from []) q($T)
+    let twf ← checkTm q($axioms) q(⟨$wf_axioms⟩) q([]) q($l) q($vT) q($t)
+    let value : Q(CheckedDef $axioms) := q(
+      have : Fact ($axioms).Wf := ⟨$wf_axioms⟩
+      { l := $l
+        tp := $T
+        nfTp := $vT
+        wf_nfTp := $vTeq .nil <| $Twf .nil
+        val := $t
+        wf_val := $twf .nil <| $vTeq .nil <| $Twf .nil
+      }
+    )
+
+    addDecl <| .defnDecl {
+      name := ci.name
+      levelParams := []
+      type := q(CheckedDef $axioms)
+      value
+      hints := .regular 0 -- TODO: what height?
+      safety := .safe
+    }
+
+    saveShallowTheoryConst thyNm (.defnInfo ci)
+    setTheoryData thyNm { thyData with env := thyEnv' }
+
+/-- Declare a new Leanternal theory with the given name.
+Theories start off with no axioms or definitions.
+You can add these using `<theory> def` and `<theory> axiom`,
+where `<theory>` is your chosen name. -/
+elab "declare_theory " thy:ident : command => do
+  let thyNm := thy.getId
+  saveTheoryDecl thyNm
+  let pre : TSyntax `str := quote s!"{thyNm} "
+  -- Bug: `command` written directly inside the quotation is hygienized,
+  -- and then the quoted command fails to run.
+  let cmdId : Ident := mkIdent `command
+  elabCommand <| ← `(command|
+    -- TODO: this makes `thyNm` a keyword token; not great?
+    elab $pre:str cmd:command : $cmdId:ident => do
+      match cmd.raw[0].getKind with
+      | `«#check» | `«#print» =>
+        let thyData ← getTheoryData $(quote thyNm)
+        withEnv thyData.env <| elabCommand cmd
+        return
+      | _ => pure ()
+
+      match cmd.raw[1].getKind with
+      | ``Parser.Command.definition => elabDeclaration $(quote thyNm) cmd
+      | ``Parser.Command.axiom => elabAxiom $(quote thyNm) cmd
+      | _ => throwError "unhandled command:{indentD cmd}"
+  )
+
+end Leanternal
