GroupoidModel/Syntax/Frontend/Prelude.lean
@@ -1,0 +1,18 @@
+prelude
+public import Init.Core
+
+/-! ## Leanternal prelude
+
+The prelude of every Leanternal theory.
+
+This imports part of the default Lean prelude,
+including definitions that we don't support (e.g. `Prop`-valued `Eq`),
+because it's difficult to make Lean function without that. -/
+
+universe u
+
+/-- The identity type. -/
+inductive Id {α : Type u} : α → α → Type u where
+  | refl (a : α) : Id a a
+
+@[match_pattern] def Id.rfl {α : Type u} {a : α} : Id a a := Id.refl a
